src/Sound/Semantics/Omni.dfy
@@ -7,9 +7,19 @@ module Omni {
       Continuation, Continuation.Update, Continuation.UpdateAndAdd, Continuation.head, Continuation.Leq,
       Continuation.UpdateHead
 
+  // Q: how to overcome the type error here?
+  // function Cons(post: iset<State>, posts: seq<iset<State>>): Continuation {
+  //   var x: Continuation := [post] + posts;
+  //   x
+  // }
+
   newtype Continuation = s : seq<iset<State>> | |s| > 0 witness [iset{}] {
 
     ghost const head : iset<State> := this[0]
+
+    function Cons(post: iset<State>): Continuation {
+      [post] + this
+    }
 
     ghost function UpdateHead(post: iset<State>): Continuation {
       this[0 := post]
@@ -57,7 +67,7 @@ module Omni {
 
    */
 
-  ghost predicate SemSingle(s: Stmt, st: State, post: iset<State>) 
+  greatest predicate SemSingle/*[nat]*/(s: Stmt, st: State, post: iset<State>) 
     requires s.Single()
   {
     match s
@@ -73,7 +83,7 @@ module Omni {
       && st[x := st.Eval(v)] in post
   }
 
-  ghost predicate Sem(s: Stmt, st: State, posts: Continuation) {
+  greatest predicate Sem/*[nat]*/(s: Stmt, st: State, posts: Continuation) {
     if s.Single() then SemSingle(s, st, posts.head) else
     match s
     case Seq(ss)        => SeqSem(ss, st, posts)
@@ -81,13 +91,17 @@ module Omni {
     case NewScope(n, s) => 
       forall vs: State :: |vs| == n ==> Sem(s, st.Update(vs), posts.UpdateAndAdd(n))
     case Escape(l)      => |posts| > l && st in posts[l]
+    case Loop(inv, body) => 
+      && inv.IsDefinedOn(|st|)
+      && st.Eval(inv)
+      && Sem(Seq([body, Loop(inv, body)]), st, posts)
   }
 
   ghost function WP(s: Stmt, posts: Continuation) : iset<State> {
     iset st: State | Sem(s, st, posts)
   }
 
-  ghost predicate SeqSem(ss: seq<Stmt>, st: State, posts: Continuation) {
+  greatest predicate SeqSem/*[nat]*/(ss: seq<Stmt>, st: State, posts: Continuation) {
     if ss == [] then st in posts.head else
     forall post': iset<State> :: 
       (forall st: State :: SeqSem(ss[1..], st, posts) ==> st in post') ==> Sem(ss[0], st, posts.UpdateHead(post'))
@@ -97,7 +111,7 @@ module Omni {
     iset st: State | SeqSem(ss, st, cont)
   }
 
-  lemma SemCons(s: Stmt, st: State, posts: Continuation, posts': Continuation)
+  greatest lemma SemCons/*[nat]*/(s: Stmt, st: State, posts: Continuation, posts': Continuation)
     requires Sem(s, st, posts)
     requires posts.Leq(posts')
     ensures Sem(s, st, posts')
@@ -108,7 +122,7 @@ module Omni {
     case _ =>
   }
 
-  lemma SeqSemCons(ss: seq<Stmt>, st: State, posts: Continuation, posts': Continuation)
+  greatest lemma SeqSemCons(ss: seq<Stmt>, st: State, posts: Continuation, posts': Continuation)
     requires SeqSem(ss, st, posts)
     requires posts.Leq(posts')
     ensures SeqSem(ss, st, posts')
@@ -120,7 +134,8 @@ module Omni {
       }
     }
   }
-  lemma SemNest(s: Stmt, ss: seq<Stmt>, st: State, posts: Continuation) 
+
+  greatest lemma SemNest(s: Stmt, ss: seq<Stmt>, st: State, posts: Continuation) 
     requires Sem(s, st, posts.UpdateHead(SeqWP(ss, posts)))
     ensures SeqSem([s] + ss, st, posts)
   {
@@ -137,6 +152,7 @@ module Omni {
     assert [s][1..] == [];
     assert posts == posts.UpdateHead(posts.head);
   }
+
 
   lemma SeqSemNest(ss1: seq<Stmt>, ss2: seq<Stmt>, st: State, posts: Continuation) 
     requires SeqSem(ss1 + ss2, st, posts)
@@ -158,4 +174,240 @@ module Omni {
     SeqSemNest(ss1, ss2, st, posts);
     SemNest(Seq(ss1), ss2, st, posts);
   }
+
+  function StateSize(st: State): nat {
+    |st|
+  }
+
+  greatest lemma SemSeqLemma(ss: seq<Stmt>, st: State, posts: Continuation)
+    requires SeqSem(ss, st, posts)
+    ensures Sem(Seq(ss), st, posts)
+  {
+
+  }
+
+  lemma SeqSemSingle'(s: Stmt, st: State, posts: Continuation)
+    requires Sem(s, st, posts)
+    ensures SeqSem([s], st, posts)
+  {
+    assert [s][0] == s;
+    assert [s][1..] == [];
+    assert posts.UpdateHead(posts.head) == posts;
+    forall post': iset<State> | (forall st: State :: SeqSem([], st, posts) ==> st in post') 
+      ensures Sem(s, st, posts.UpdateHead(post')) {
+      SemCons(s, st, posts, posts.UpdateHead(post'));
+    }
+  }
+
+  lemma SemSeqLemmak(k: ORDINAL, ss: seq<Stmt>, st: State, posts: Continuation)
+    // requires k.Offset > 0
+    requires SeqSem#[k](ss, st, posts)
+    // ensures Sem#[k+1](Seq(ss), st, posts)
+    ensures Sem#[k](Seq(ss), st, posts)
+  {
+
+  }
+
+  ghost function SeqWPk(k: ORDINAL, ss: seq<Stmt>, cont: Continuation): iset<State> {
+    iset st: State | SeqSem#[k](ss, st, cont)
+  }
+
+  lemma SemNestk(k: ORDINAL, s: Stmt, ss: seq<Stmt>, st: State, posts: Continuation) 
+    requires Sem#[k](s, st, posts.UpdateHead(SeqWPk(k, ss, posts)))
+    ensures SeqSem#[k]([s] + ss, st, posts)
+  {
+    // forall post': iset<State> | (forall st: State :: SeqSem(ss, st, posts) ==> st in post') {
+    //   SemCons(s, st, posts.UpdateHead(SeqWP(ss, posts)), posts.UpdateHead(post'));
+    // }
+  }
+
+  lemma SemConsk/*[nat]*/(k: ORDINAL, s: Stmt, st: State, posts: Continuation, posts': Continuation)
+    requires Sem#[k](s, st, posts)
+    requires posts.Leq(posts')
+    ensures Sem#[k](s, st, posts')
+  {
+    // match s
+    // case Seq(ss) => SeqSemCons(ss, st, posts, posts');
+    // case NewScope(n, s) => posts.LeqUpdateAndAdd(n, posts');
+    // case _ =>
+  }
+
+  lemma SeqSemSingle'k(k: ORDINAL, s: Stmt, st: State, posts: Continuation)
+    requires Sem#[k](s, st, posts)
+    ensures SeqSem#[k]([s], st, posts)
+  {
+    // assert [s][0] == s;
+    // assert [s][1..] == [];
+    // assert posts.UpdateHead(posts.head) == posts;
+    // forall post': iset<State> | (forall st: State :: SeqSem([], st, posts) ==> st in post') 
+    //   ensures Sem(s, st, posts.UpdateHead(post')) {
+    //   SemCons(s, st, posts, posts.UpdateHead(post'));
+    // }
+  }
+  /**
+    (st, Loop(body)) ===> posts
+
+    |-
+
+    exists inv', 
+      && forall st <- inv' :: Sem(body, st, posts.Cons(inv'))
+
+  
+  inv' := iset st': State | 
+    exists n, 
+      forall post', 
+        SeqSem(SeqOf(n, body), st, posts.Cons(post')) ==> st' in post'
+  
+   */
+
+  lemma SemLoopk(k: ORDINAL, inv: Expr, body: Stmt, st: State, posts: Continuation)
+    requires forall st <- inv.Sem() :: Sem(body, st, posts.Cons(inv.Sem()))
+    requires st in inv.Sem()
+    ensures Sem#[k](Loop(inv, body), st, posts.Cons(inv.Sem()))
+    decreases k
+  {
+    if k.Offset > 0 {
+    assert inv.IsDefinedOn(StateSize(st)) && st.Eval(inv); 
+    assert Sem#[k - 1](Seq([body, Loop(inv, body)]), st, posts.Cons(inv.Sem())) by {
+      SemSeqLemmak(k - 1, [body, Loop(inv, body)], st, posts.Cons(inv.Sem())) by {
+        assert SeqSem#[k - 1]([body, Loop(inv, body)], st, posts.Cons(inv.Sem())) by {
+          assert [body] + [Loop(inv, body)] == [body, Loop(inv, body)];
+          SemNestk(k - 1,body, [Loop(inv, body)], st, posts.Cons(inv.Sem())) by {
+            assert 
+              posts.Cons(inv.Sem()).UpdateHead(SeqWPk(k - 1, [Loop(inv, body)], posts.Cons(inv.Sem()))) ==
+              posts.Cons(SeqWPk(k - 1, [Loop(inv, body)], posts.Cons(inv.Sem())));
+            assert inv.Sem() <= SeqWPk(k - 1, [Loop(inv, body)], posts.Cons(inv.Sem())) by {
+              forall st | st in inv.Sem() 
+                ensures st in SeqWPk(k - 1, [Loop(inv, body)], posts.Cons(inv.Sem())) {
+                  SeqSemSingle'k(k - 1, Loop(inv, body), st, posts.Cons(inv.Sem())) by {
+                    assert Sem#[k - 1](Loop(inv, body), st, posts.Cons(inv.Sem())) by {
+                    SemLoopk(k - 1, inv, body, st, posts);
+                  }
+                }
+              }
+            }
+            SemConsk(k - 1, body, st, posts.Cons(inv.Sem()), posts.Cons(SeqWPk(k - 1, [Loop(inv, body)], posts.Cons(inv.Sem()))));
+          }
+        }
+      }
+    }
+  }
+  }
+
+  // lemma SeqSemSingle'k(k: ORDINAL, s: Stmt, st: State, posts: Continuation)
+  //   requires Sem#[k](s, st, posts)
+  //   ensures SeqSem#[k]([s], st, posts)
+  // {
+  //   // SemNestk(k, s, [], st, posts);
+  // }
+
+  // lemma SemConsk/*[nat]*/(k: ORDINAL, s: Stmt, st: State, posts: Continuation, posts': Continuation)
+  //   requires Sem#[k](s, st, posts)
+  //   requires posts.Leq(posts')
+  //   ensures Sem#[k](s, st, posts')
+  // {
+  //   // match s
+  //   // case Seq(ss) => SeqSemConsk(k, ss, st, posts, posts');
+  //   // case NewScope(n, s) => posts.LeqUpdateAndAdd(n, posts');
+  //   // case _ =>
+  // }
+
+  // lemma SemSeqLemmak(k: ORDINAL, ss: seq<Stmt>, st: State, posts: Continuation)
+  //   requires SeqSem#[k](ss, st, posts)
+  //   ensures Sem#[k](Seq(ss), st, posts)
+  // {
+
+  // }
+
+  // lemma SemNestk(k: ORDINAL, s: Stmt, ss: seq<Stmt>, st: State, posts: Continuation) 
+  //   requires Sem#[k](s, st, posts.UpdateHead(SeqWPk(k, ss, posts)))
+  //   ensures SeqSem#[k]([s] + ss, st, posts)
+  // {
+  //   forall post': iset<State> | (forall st: State :: SeqSem#[k](ss, st, posts) ==> st in post') {
+  //     SemConsk(k, s, st, posts.UpdateHead(SeqWPk(k, ss, posts)), posts.UpdateHead(post'));
+  //   }
+  // }
+
+  // ghost function SeqWPk(k: ORDINAL, ss: seq<Stmt>, cont: Continuation): iset<State> {
+  //   iset st: State | SeqSem#[k](ss, st, cont)
+  // }
+
+  // greatest lemma InSeqWPLemma(k: ORDINAL, ss: seq<Stmt>, st: State, posts: Continuation)
+  //   requires SeqSem#[k](ss, st, posts)
+  //   ensures st in SeqWPk(k, ss, posts)
+  // { 
+
+  // }
+
+  // lemma SemLoop(k: ORDINAL, inv: Expr, body: Stmt, st: State, posts: Continuation)
+  //   requires forall st <- inv.Sem() :: Sem#[k](body, st, posts.Cons(inv.Sem()))
+  //   requires st in inv.Sem()
+  //   ensures Sem#[k](Loop(inv, body), st, posts.Cons(inv.Sem()))
+  // {
+  //   assert inv.IsDefinedOn(StateSize(st)) && st.Eval(inv); 
+  //   assert Sem#[k - 1](Seq([body, Loop(inv, body)]), st, posts.Cons(inv.Sem())) by {
+  //     SemSeqLemma#[k - 1]([body, Loop(inv, body)], st, posts.Cons(inv.Sem())) by {
+  //       // BUG: this is not working
+  //       assert SeqSem#[k - 1]([body, Loop(inv, body)], st, posts.Cons(inv.Sem())) by {
+  //         assert [body] + [Loop(inv, body)] == [body, Loop(inv, body)];
+  //         SemNestk(k - 1, body, [Loop(inv, body)], st, posts.Cons(inv.Sem())) by {
+  //           assert 
+  //             posts.Cons(inv.Sem()).UpdateHead(SeqWPk(k - 1, [Loop(inv, body)], posts.Cons(inv.Sem()))) ==
+  //             posts.Cons(SeqWPk(k - 1, [Loop(inv, body)], posts.Cons(inv.Sem())));
+  //           assert inv.Sem() <= SeqWPk(k - 1, [Loop(inv, body)], posts.Cons(inv.Sem())) by {
+  //             forall st | st in inv.Sem() 
+  //               ensures st in SeqWPk(k - 1, [Loop(inv, body)], posts.Cons(inv.Sem())) {
+  //               InSeqWPLemma(k - 1, [Loop(inv, body)], st, posts.Cons(inv.Sem())) by {
+  //                 SeqSemSingle'k(k - 1, Loop(inv, body), st, posts.Cons(inv.Sem())) by {
+  //                   SemLoop(k - 1, inv, body, st, posts);
+  //                 }
+  //               }
+  //             }
+  //           }
+  //           SemConsk(k - 1, body, st, posts.Cons(inv.Sem()), posts.Cons(SeqWPk(k - 1, [Loop(inv, body)], posts.Cons(inv.Sem()))));
+  //         }
+  //       }
+  //     }
+  //   }
+  // }
+  
+
+  greatest lemma SemLoop(inv: Expr, body: Stmt, st: State, posts: Continuation)
+    requires forall st <- inv.Sem() :: Sem(body, st, posts.Cons(inv.Sem())) // [inv.Sem()] + posts
+    requires st in inv.Sem()
+    ensures Sem(Loop(inv, body), st, posts.Cons(iset{}))
+  // {
+  //   assert inv.IsDefinedOn(StateSize(st)) && st.Eval(inv); 
+  //   assert Sem(Seq([body, Loop(inv, body)]), st, posts.Cons(inv.Sem())) by {
+  //     SemSeqLemma([body, Loop(inv, body)], st, posts.Cons(inv.Sem())) by {
+  //       // BUG: this is not working
+  //       // assert SeqSem([body, Loop(inv, body)], st, posts.Cons(inv.Sem())) by {
+  //         assert [body] + [Loop(inv, body)] == [body, Loop(inv, body)];
+  //         SemNest(body, [Loop(inv, body)], st, posts.Cons(inv.Sem())) by {
+  //           assert 
+  //             posts.Cons(inv.Sem()).UpdateHead(SeqWP([Loop(inv, body)], posts.Cons(inv.Sem()))) ==
+  //             posts.Cons(SeqWP([Loop(inv, body)], posts.Cons(inv.Sem())));
+  //           assert inv.Sem() <= SeqWP([Loop(inv, body)], posts.Cons(inv.Sem())) by {
+  //             forall st | st in inv.Sem() 
+  //               ensures st in SeqWP([Loop(inv, body)], posts.Cons(inv.Sem())) {
+  //                 SeqSemSingle'(Loop(inv, body), st, posts.Cons(inv.Sem())) by {
+  //                   assert Sem(Loop(inv, body), st, posts.Cons(inv.Sem())) by {
+  //                   SemLoop(inv, body, st, posts);
+  //                 }
+  //               }
+  //             }
+  //           }
+  //           SemCons(body, st, posts.Cons(inv.Sem()), posts.Cons(SeqWP([Loop(inv, body)], posts.Cons(inv.Sem()))));
+  //         }
+  //     }
+  //   }
+  // }
+
+  // lemma SemLoop(inv: Expr, body: Stmt, st: State, posts: Continuation)
+  //   ensures Sem(body, st, posts.UpdateHead(SeqWP([body, Loop(inv, body)], posts)))
+  //   requires Sem(Loop(inv, body), st, posts)
+  // // {
+
+  // // }
+  
 }
